Try ranged approach

Regex/NFA/Compile.lean
@@ -67,9 +67,6 @@ where
     Returned NFA contains the compiled nodes at the end and starts at the node
     corresponding to the given regex.
   -/
-  -- TODO: now I don't think we use NFA's ordering except for the size inequality.
-  -- Just replace the condition.
-  -- TODO: check all array insertions are handled linearly.
   loop (r : Regex) (next : Nat) (nfa : NFA) : { nfa' // nfa ≤ nfa' } := match r with
   | .empty => nfa.addNode .fail
   | .epsilon => nfa.addNode (.epsilon next)
@@ -101,53 +98,47 @@ where
     ⟨nfa₁, property⟩
   | .star r =>
     -- We need to generate a placeholder node first. We use `fail` for it because
-    -- 1. We want to make sure `done` does not appear except at the first node.
-    -- 2. variants without data are represented as a boxed integer so there is one less allocation.
+    -- 1. We'll use the fact that `fail` is a minimal element when strengthening induction hypotheis;
+    -- 2. We want to make sure `done` does not appear except at the first node.
+    -- 3. variants without data are represented as a boxed integer so there is one less allocation.
     -- TODO: check generated code
-    let placeholder := nfa.addNode .fail
-    let loopStart := placeholder.val.start
-    let compiled := loop r loopStart placeholder
+    let nfa' := nfa.addNode .fail
+    let start := nfa'.val.start
+    let nfa'' := loop r start nfa'
 
-    -- have property : nfa ≤ compiled :=
-    --   calc nfa
-    --     _ ≤ placeholder.val := placeholder.property
-    --     _ ≤ compiled.val := compiled.property
-    have isLt : loopStart.val < compiled.val.nodes.size :=
-      Nat.lt_of_lt_of_le placeholder.val.start.isLt (NFA.le_size_of_le compiled.property)
+    have property : nfa ≤ nfa'' :=
+      calc nfa
+        _ ≤ nfa'.val := nfa'.property
+        _ ≤ nfa''.val := nfa''.property
+    have isLt : start.val < nfa''.val.nodes.size :=
+      Nat.lt_of_lt_of_le nfa'.val.start.isLt (NFA.le_size_of_le nfa''.property)
 
     -- Patch the placeholder node
-    let target := compiled.val.start
-    let nodes := compiled.val.nodes.set ⟨loopStart.val, isLt⟩ (.split target next)
+    let target := nfa''.val.start
+    let nodes''' := nfa''.val.nodes.set ⟨start.val, isLt⟩ (.split target next)
 
-    have eq_size : nodes.size = compiled.val.nodes.size := by simp
-    have isLt' : loopStart.val < nodes.size := eq_size ▸ isLt
-    let patched : NFA := ⟨nodes, ⟨loopStart.val, isLt'⟩⟩
+    have eq_size : nodes'''.size = nfa''.val.nodes.size := by simp
+    have isLt' : start.val < nodes'''.size := eq_size ▸ isLt
+    let nfa''' := ⟨nodes''', ⟨start.val, isLt'⟩⟩
 
-    -- Add the start node
-    -- Creating a split node with the same targets feels a bit waste
-    let final := patched.addNode (.split loopStart loopStart)
-
-    have property' : nfa ≤ final := by
+    have property' : nfa ≤ nfa''' := by
       intro i h
 
-      -- have le_size : nfa.nodes.size ≤ nfa''.val.nodes.size := NFA.le_size_of_le property
-      -- have h₂ : i < nodes.size := Nat.lt_of_lt_of_le h (eq_size ▸ le_size)
-      have h₂ : i < final.val.nodes.size := sorry
+      have le_size : nfa.nodes.size ≤ nfa''.val.nodes.size := NFA.le_size_of_le property
+      have h₂ : i < nodes'''.size := Nat.lt_of_lt_of_le h (eq_size ▸ le_size)
       exists h₂
 
-      -- have eq : nfa'''[i] = nfa''.val[i]'(Nat.lt_of_lt_of_le h le_size) := by
-      --   apply Array.get_set_ne
-      --   exact (Nat.ne_of_gt h)
-      -- rw [eq]
-      -- exact (property i _).2
-      sorry
+      have eq : nfa'''[i] = nfa''.val[i]'(Nat.lt_of_lt_of_le h le_size) := by
+        apply Array.get_set_ne
+        exact (Nat.ne_of_gt h)
+      rw [eq]
+      exact (property i _).2
 
-    ⟨final, property'⟩
+    ⟨nfa''', property'⟩
 
 #eval compile (Regex.star (Regex.char 'a'))
 #eval compile (Regex.alternate (Regex.char 'x') (Regex.star (Regex.concat (Regex.char 'a') (Regex.char 'b'))))
 #eval compile (Regex.alternate Regex.empty (Regex.concat (Regex.char 'a') Regex.empty))
-#eval compile (Regex.concat (Regex.star (Regex.char 'a')) (Regex.star (Regex.char 'b')))
 
 -- Useful lemmas about the compilation
 theorem compile.loop.le : nfa ≤ (compile.loop r next nfa).val :=
@@ -214,41 +205,49 @@ theorem compile.loop.concat (eq : compile.loop (Regex.concat r₁ r₂) next nfa
   exact motive nfa₂ nfa₁ property rfl rfl this
 
 theorem compile.loop.star (eq : compile.loop (Regex.star r) next nfa = result)
-  {motive : ∀placeholder loopStart compiled nodes patched final isLt isLt' property',
-    placeholder = nfa.addNode .fail →
-    loopStart = placeholder.val.start →
-    compiled = compile.loop r loopStart placeholder →
-    nodes = compiled.val.nodes.set ⟨loopStart.val, isLt⟩ (.split compiled.val.start next) →
-    patched = NFA.mk nodes ⟨loopStart.val, isLt'⟩ →
-    final = patched.addNode (.split loopStart loopStart) →
-    result = ⟨final, property'⟩ →
+  {motive : ∀nfa' start nfa'' nodes''' nfa''' isLt isLt' property',
+    nfa' = nfa.addNode .fail →
+    start = nfa'.val.start →
+    nfa'' = compile.loop r start nfa' →
+    nodes''' = nfa''.val.nodes.set ⟨start.val, isLt⟩ (.split nfa''.val.start next) →
+    nfa''' = ⟨nodes''', ⟨start.val, isLt'⟩⟩ →
+    result = ⟨nfa''', property'⟩ →
     P
   } : P := by
-  let placeholder := nfa.addNode .fail
-  let loopStart := placeholder.val.start
-  let compiled := loop r loopStart placeholder
+  let nfa' := nfa.addNode .fail
+  let start := nfa'.val.start
+  let nfa'' := loop r start nfa'
 
-  have isLt : loopStart.val < compiled.val.nodes.size :=
-    Nat.lt_of_lt_of_le placeholder.val.start.isLt (NFA.le_size_of_le compiled.property)
+  have property : nfa ≤ nfa'' :=
+    calc nfa
+      _ ≤ nfa'.val := nfa'.property
+      _ ≤ nfa''.val := nfa''.property
+  have isLt : start.val < nfa''.val.nodes.size :=
+    Nat.lt_of_lt_of_le nfa'.val.start.isLt (NFA.le_size_of_le nfa''.property)
 
   -- Patch the placeholder node
-  let target := compiled.val.start
-  let nodes := compiled.val.nodes.set ⟨loopStart.val, isLt⟩ (.split target next)
+  let nodes''' := nfa''.val.nodes.set ⟨start.val, isLt⟩ (.split nfa''.val.start next)
 
-  have eq_size : nodes.size = compiled.val.nodes.size := by simp
-  have isLt' : loopStart.val < nodes.size := eq_size ▸ isLt
-  let patched : NFA := ⟨nodes, ⟨loopStart.val, isLt'⟩⟩
+  have eq_size : nodes'''.size = nfa''.val.nodes.size := by simp
+  have isLt' : start.val < nodes'''.size := eq_size ▸ isLt
+  let nfa''' : NFA := ⟨nodes''', ⟨start.val, isLt'⟩⟩
 
-  -- Add the start node
-  -- Creating a split node with the same targets feels a bit waste
-  let final := patched.addNode (.split loopStart loopStart)
+  have property' : nfa ≤ nfa''' := by
+    intro i h
 
-  have property' : nfa ≤ final := sorry
+    have le_size : nfa.nodes.size ≤ nfa''.val.nodes.size := NFA.le_size_of_le property
+    have h₂ : i < nodes'''.size := Nat.lt_of_lt_of_le h (eq_size ▸ le_size)
+    exists h₂
 
-  have : result = ⟨final, property'⟩ := by
+    have eq : nfa'''[i] = nfa''.val[i]'(Nat.lt_of_lt_of_le h le_size) := by
+      apply Array.get_set_ne
+      exact (Nat.ne_of_gt h)
+    rw [eq]
+    exact (property i _).2
+
+  have : result = ⟨nfa''', property'⟩ := by
     simp [eq.symm, compile.loop]
-  exact motive placeholder loopStart compiled nodes patched final isLt isLt' property'
-    rfl rfl rfl rfl rfl rfl this
+  exact motive nfa' start nfa'' nodes''' nfa''' isLt isLt' property' rfl rfl rfl rfl rfl this
 
 theorem compile.loop.get_lt (eq : compile.loop r next nfa = result)
   (h : i < nfa.nodes.size) :
@@ -285,29 +284,24 @@ theorem compile.loop.get_lt (eq : compile.loop r next nfa = result)
     simp [ih₂ eq₂.symm h]
   | star r ih =>
     apply compile.loop.star eq
-    intro placeholder loopStart compiled nodes patched final isLt isLt' property'
-      eq₁ eq₂ eq₃ eq₄ eq₅ eq₆ eq
+    intro nfa' start nfa'' nodes''' nfa''' isLt isLt' property'
+      eq₁ eq₂ eq₃ eq₄ eq₅ eq
 
-    have h' : i < placeholder.val.nodes.size :=
-      Nat.lt_of_lt_of_le h (NFA.le_size_of_le placeholder.property)
-    have h'' : i < compiled.val.nodes.size :=
-      Nat.lt_of_lt_of_le h' (NFA.le_size_of_le compiled.property)
-    have h''' : i < patched.nodes.size := by
-      simp [eq₅, eq₄]
-      exact h''
-    have ne : (Fin.mk loopStart isLt).val ≠ i := by
+    have h' : i < nfa'.val.nodes.size :=
+      Nat.lt_of_lt_of_le h (NFA.le_size_of_le nfa'.property)
+    have h'' : i < nfa''.val.nodes.size :=
+      Nat.lt_of_lt_of_le h' (NFA.le_size_of_le nfa''.property)
+    have ih := ih eq₃.symm h'
+    have ne : (Fin.mk start isLt).val ≠ i := by
       simp [eq₂]
       rw [eq₁]
       simp [NFA.addNode]
       exact Nat.ne_of_gt h
-    have ih := ih eq₃.symm h'
 
     conv =>
       lhs
-      simp [eq, eq₆, eq₅]
-      rw [NFA.get_lt_addNode h''', NFA.eq_get]
-      simp [eq₅, eq₄]
-      rw [Array.get_set_ne compiled.val.nodes ⟨loopStart, isLt⟩ _ h'' ne]
+      simp [eq, eq₅, NFA.eq_get, eq₄]
+      rw [Array.get_set_ne nfa''.val.nodes ⟨start, isLt⟩ _ h'' ne]
       simp [NFA.eq_get.symm, ih]
       simp [eq₁, NFA.get_lt_addNode h]
 
@@ -357,10 +351,10 @@ theorem compile.loop.get_done_of_zero (eq : compile.loop r next nfa = result)
     apply ih₂ eq₂.symm assm
   | star r ih =>
     apply compile.loop.star eq
-    intro placeholder loopStart compiled nodes patched final isLt isLt' property'
-      eq₁ _ eq₃ eq₄ eq₅ eq₆ eq i h done
+    intro nfa' start nfa'' nodes''' nfa''' isLt isLt' property'
+      eq₁ _ eq₃ eq₄ eq₅ eq i h done
 
-    have assm' : ∀i, (_ : i < placeholder.val.nodes.size) → placeholder.val[i] = .done → i = 0 := by
+    have assm' : ∀i, (_ : i < nfa'.val.nodes.size) → nfa'.val[i] = .done → i = 0 := by
       intro i h done
       cases Nat.lt_or_ge i nfa.nodes.size with
       | inl lt =>
@@ -370,28 +364,15 @@ theorem compile.loop.get_done_of_zero (eq : compile.loop r next nfa = result)
         simp [eq₁, NFA.addNode] at h
         have : i = nfa.nodes.size := Nat.eq_of_ge_of_lt ge h
         simp [this, eq₁] at done
-    cases Nat.lt_or_ge i compiled.val.nodes.size with
-    | inl h' =>
-      have h'' : i < patched.nodes.size := by
-        simp [eq₅, eq₄]
-        exact h'
-      have ih := ih eq₃.symm assm' i h'
+    have h' : i < nfa''.val.nodes.size := by
+      simp [eq, eq₅, eq₄] at h
+      exact h
+    have ih := ih eq₃.symm assm' i h'
 
-      simp [eq, eq₆] at done
-      have done : patched[i] = .done := by
-        rw [NFA.get_lt_addNode h''] at done
-        exact done
-      simp [eq₅, NFA.eq_get, eq₄, Array.get_set, h'] at done
-      split at done
-      . exact done.elim
-      . exact ih done
-    | inr ge =>
-      simp [eq, eq₆, NFA.addNode, eq₅, eq₄] at h
-      have : i = compiled.val.nodes.size := Nat.eq_of_ge_of_lt ge h
-      have : i = patched.nodes.size := by
-        simp [eq₅, eq₄]
-        exact this
-      simp [this, eq, eq₆] at done
+    simp [eq, eq₅, NFA.eq_get, eq₄, Array.get_set, h'] at done
+    split at done
+    . exact done.elim
+    . exact ih done
 
 theorem compile.get_done_iff_zero (eq : compile r = result) (h : i < result.nodes.size) :
   result[i] = .done ↔ i = 0 := by
@@ -473,10 +454,16 @@ theorem compile.loop.inBounds (eq : compile.loop r next nfa = result)
     apply ih₂ eq₂.symm h₁ h₂
   | star r ih =>
     apply compile.loop.star eq
-    intro placeholder loopStart compiled nodes patched final isLt isLt' property'
-      eq₁ _ eq₃ eq₄ eq₅ eq₆ eq i
+    intro nfa' start nfa'' nodes''' nfa''' isLt isLt' property'
+      eq₁ _ eq₃ eq₄ eq₅ eq i
 
-    have inBounds' : placeholder.val.inBounds := by
+    have eqsize : result.val.nodes.size = nfa''.val.nodes.size := by
+      simp [eq, eq₅, eq₄]
+    have h' : i < nfa''.val.nodes.size :=
+      calc
+        i < result.val.nodes.size := i.isLt
+        _ = _ := eqsize
+    have inBounds' : nfa'.val.inBounds := by
       simp [eq₁]
       intro i
       cases Nat.lt_or_ge i nfa.nodes.size with
@@ -488,129 +475,14 @@ theorem compile.loop.inBounds (eq : compile.loop r next nfa = result)
         simp only [NFA.addNode, Array.size_push] at lt
         have : i = nfa.nodes.size := Nat.eq_of_ge_of_lt ge lt
         simp [this]
-    have ih := ih eq₃.symm loopStart.isLt inBounds'
+    have ih := ih eq₃.symm start.isLt inBounds'
 
-    cases Nat.lt_or_ge i patched.nodes.size with
-    | inl lt =>
-      have hj : i < compiled.val.nodes.size := by
-        simp [eq₅, eq₄] at lt
-        exact lt
-      have : result.val[i] = patched.nodes[i] := by
-        simp [eq, eq₆, NFA.get_lt_addNode lt]
-        exact NFA.eq_get
-      rw [this]
-      simp [eq₅, eq₄]
-      rw [Array.get_set _ _ _ hj]
-      have h' : compiled.val.nodes.size ≤ result.val.nodes.size := by
-        simp [eq, eq₆, NFA.addNode, eq₅, eq₄]
-        exact Nat.le_succ _
-      split
-      . apply Node.inBounds.split
-        . calc compiled.val.start.val
-            _ < compiled.val.nodes.size := compiled.val.start.isLt
-            _ ≤ _ := h'
-        . calc next
-            _ < nfa.nodes.size := h₁
-            _ ≤ placeholder.val.nodes.size := NFA.le_size_of_le placeholder.property
-            _ ≤ compiled.val.nodes.size := NFA.le_size_of_le compiled.property
-            _ ≤ _ := h'
-      . exact Node.inBounds_of_inBounds_of_le (ih ⟨i, hj⟩) h'
-    | inr ge =>
-      have h : loopStart < patched.nodes.size + 1 :=
-        calc loopStart.val
-          _ < placeholder.val.nodes.size := loopStart.isLt
-          _ ≤ compiled.val.nodes.size := NFA.le_size_of_le compiled.property
-          _ = patched.nodes.size := by simp [eq₅, eq₄]
-          _ < _ := Nat.lt_succ_self _
-      have lt : i < patched.nodes.size + 1 := by
-        have : i < result.val.nodes.size := i.isLt
-        simp [eq, eq₆, NFA.addNode] at this
-        exact this
-      have : i = patched.nodes.size := Nat.eq_of_ge_of_lt ge lt
-      simp [this, eq, eq₆]
-      simp [NFA.addNode]
-      apply Node.inBounds.split <;> exact h
-
-theorem compile.loop.inBounds.star.compiled {i : Nat} (eq : compile.loop (.star r) next nfa = result)
-  (h₁ : next < nfa.nodes.size) (h₂ : nfa.inBounds) (assm : i < result.val.nodes.size - 1) :
-  (result.val[i]'(Nat.lt_of_lt_of_le assm (Nat.sub_le _ _))).inBounds (result.val.nodes.size - 1) := by
-  apply compile.loop.star eq
-  intro placeholder loopStart compiled nodes patched final isLt isLt' property'
-    eq₁ _ eq₃ eq₄ eq₅ eq₆ eq
-
-  have inBounds' : placeholder.val.inBounds := by
-    simp [eq₁]
-    intro i
-    cases Nat.lt_or_ge i nfa.nodes.size with
-    | inl lt =>
-      simp [NFA.get_lt_addNode lt]
-      exact Node.inBounds_of_inBounds_of_le (h₂ ⟨i, lt⟩) (by simp [NFA.addNode]; exact Nat.le_succ _)
-    | inr ge =>
-      let lt := i.isLt
-      simp only [NFA.addNode, Array.size_push] at lt
-      have : i = nfa.nodes.size := Nat.eq_of_ge_of_lt ge lt
-      simp [this]
-  have inBounds'' := compile.loop.inBounds eq₃.symm loopStart.isLt inBounds'
-
-  have size : result.val.nodes.size - 1 = compiled.val.nodes.size := by
-    simp [eq, eq₆, NFA.addNode, eq₅, eq₄]
-  have assm' : i < compiled.val.nodes.size := size ▸ assm
-  simp [size]
-
-  simp [eq, eq₆]
-  have : i < patched.nodes.size := by
-    simp [eq₅, eq₄]
-    exact assm'
-  rw [NFA.get_lt_addNode this]
-  simp [eq₅, NFA.eq_get, eq₄, Array.get_set (hj := assm')]
-  split
-  . apply Node.inBounds.split
-    . exact compiled.val.start.isLt
-    . calc next
-        _ < nfa.nodes.size := h₁
-        _ ≤ placeholder.val.nodes.size := NFA.le_size_of_le placeholder.property
-        _ ≤ compiled.val.nodes.size := NFA.le_size_of_le compiled.property
-  . exact inBounds'' ⟨i, assm'⟩
-
-theorem compile.loop.start (eq : compile.loop r next nfa = result) :
-  result.val.start.val = result.val.nodes.size - 1 := by
-  induction r generalizing next nfa with
-  | empty =>
-    apply compile.loop.empty eq
-    intro eq
-    rw [eq]
-    simp [NFA.addNode]
-  | epsilon =>
-    apply compile.loop.epsilon eq
-    intro eq
-    rw [eq]
-    simp [NFA.addNode]
-  | char c =>
-    apply compile.loop.char eq
-    intro eq
-    rw [eq]
-    simp [NFA.addNode]
-  | alternate r₁ r₂ =>
-    apply compile.loop.alternate eq
-    intro nfa₁ start₁ nfa₂ start₂ nfa' property _ _ _ _ eq₅ eq
-    rw [eq]
-    simp
-    rw [eq₅]
-    simp [NFA.addNode]
-  | concat r₁ r₂ ih₁ =>
-    apply compile.loop.concat eq
-    intro nfa₂ nfa₁ property _ eq₁ eq
-    rw [eq]
-    simp
-    exact ih₁ eq₁.symm
-  | star r =>
-    apply compile.loop.star eq
-    intro placeholder loopStart compiled nodes patched final isLt isLt' property'
-      _ _ _ eq₄ eq₅ eq₆ eq
-    rw [eq]
-    simp
-    rw [eq₆, eq₅]
-    simp [NFA.addNode, eq₄]
+    simp [eq, eq₅, NFA.eq_get, eq₄, Array.get_set, h']
+    split
+    . apply Node.inBounds.split
+      . exact nfa''.val.start.isLt
+      . exact Nat.lt_of_lt_of_le h₁ (NFA.le_size_of_le (le_trans nfa'.property nfa''.property))
+    . exact ih (i.cast eqsize)
 
 theorem compile.inBounds (eq : compile r = result) : result.inBounds := by
   let init : NFA := ⟨#[.done], ⟨0, Nat.zero_lt_succ _⟩⟩
@@ -664,15 +536,14 @@ theorem compile.loop.start_in_NewNodesRange (eq : compile.loop r next nfa = resu
     exact le_trans (NFA.le_size_of_le nfa₂.property) ih₁
   | star r =>
     apply compile.loop.star eq
-    intro placeholder loopStart compiled nodes patched final isLt isLt' property'
-      _ _ _ eq₄ eq₅ eq₆ eq
+    intro nfa' start nfa'' nodes''' nfa''' isLt isLt' property'
+      eq₁ eq₂ _ _ eq₅ eq
     rw [eq]
     simp
-    rw [eq₆, eq₅]
-    simp [NFA.addNode, eq₄]
-    calc nfa.nodes.size
-      _ ≤ placeholder.val.nodes.size := NFA.le_size_of_le placeholder.property
-      _ ≤ compiled.val.nodes.size := NFA.le_size_of_le compiled.property
+    rw [eq₅]
+    simp [eq₂]
+    rw [eq₁]
+    simp [NFA.addNode]
 
 theorem compile.loop.step_range (c : Char) (eq : compile.loop r next nfa = result) :
   ∀i, nfa.nodes.size ≤ i → (_ : i < result.val.nodes.size) →
@@ -796,134 +667,109 @@ theorem compile.loop.step_range (c : Char) (eq : compile.loop r next nfa = resul
       exact ⟨le_trans ih₁.left this, le_trans ih₁.right this⟩
   | star r ih =>
     apply compile.loop.star eq
-    intro placeholder loopStart compiled nodes patched final isLt isLt' property'
-      eq₁ eq₂ eq₃ eq₄ eq₅ eq₆ eq i h₁ h₂
+    intro nfa' start nfa'' nodes''' nfa''' isLt isLt' property'
+      eq₁ eq₂ eq₃ eq₄ eq₅ eq i h₁ h₂
     simp [NewNodesRange, eq]
 
-    have : i < final.val.nodes.size := by
+    have eqs : start.val = nfa.nodes.size := by
+      simp [eq₂]
+      rw [eq₁]
+      simp [NFA.addNode]
+    have size : i < nfa'''.nodes.size := by
       simp [eq] at h₂
       exact h₂
+    have eqsize : nfa''.val.nodes.size = nfa'''.nodes.size := by
+      simp [eq₅, eq₄]
+    have size'' : i < nfa''.val.nodes.size := eqsize ▸ size
 
-    cases Nat.lt_or_ge i placeholder.val.nodes.size with
+    cases Nat.lt_or_ge i nfa'.val.nodes.size with
     | inl lt =>
       simp [eq₁, NFA.addNode] at lt
       have h := Nat.eq_of_ge_of_lt h₁ lt
-      have : final.val[i] = .split compiled.val.start next := by
-        have : i = loopStart := by
-          simp [eq₂]
-          rw [eq₁]
-          simp [NFA.addNode]
-          exact h
-        simp [this, eq₆]
-        have : loopStart.val < patched.nodes.size :=
-          calc loopStart.val
-            _ < nodes.size := isLt'
-            _ = patched.nodes.size := by simp [eq₅, eq₄]
-        simp [NFA.get_lt_addNode this]
-        simp [eq₅, NFA.eq_get, eq₄]
+      have : nfa'''[i] = .split nfa''.val.start next := by
+        have : i = start := by
+          rw [h, eqs]
+        simp [this, eq₅, NFA.eq_get, eq₄]
       simp [this, Node.charStep, Node.εStep]
       apply Set.insert_subset
       . have h := start_in_NewNodesRange eq₃.symm
         simp
-        refine .inr ⟨le_trans (NFA.le_size_of_le placeholder.property) h.left, ?_⟩
-        calc compiled.val.start.val
-          _ < compiled.val.nodes.size := compiled.val.start.isLt
-          _ ≤ patched.nodes.size := by simp [eq₅, eq₄]
-          _ < _ := by simp [eq₆, NFA.addNode]
+        exact .inr ⟨le_trans (NFA.le_size_of_le nfa'.property) h.left, eqsize ▸ nfa''.val.start.isLt⟩
       . simp
     | inr ge =>
-      cases Nat.lt_or_ge i compiled.val.nodes.size with
-      | inl lt =>
-        have ih := ih eq₃.symm i ge lt
-        have : i < patched.nodes.size := by
-          simp [eq₅, eq₄]
-          exact lt
-        simp [eq₆]
-        rw [NFA.get_lt_addNode this]
-        simp [NFA.eq_get, eq₅, eq₄]
-        have ne : (Fin.mk loopStart isLt).val ≠ i := Nat.ne_of_lt (Nat.lt_of_lt_of_le loopStart.isLt ge)
-        rw [Array.get_set_ne _ _ _ lt ne]
-        simp [NFA.addNode]
-        have : {loopStart.val} ∪ NewNodesRange eq₃.symm ⊆
-          {next} ∪ {i | nfa.nodes.size ≤ i ∧ i < patched.nodes.size + 1} := by
-          apply Set.union_subset
-          . simp [eq₂]
-            rw [eq₁]
-            simp [NFA.addNode]
-            apply Or.inr
-            calc nfa.nodes.size
-              _ ≤ placeholder.val.nodes.size := NFA.le_size_of_le placeholder.property
-              _ ≤ compiled.val.nodes.size := NFA.le_size_of_le compiled.property
-              _ ≤ patched.nodes.size := by simp [eq₅, eq₄]
-              _ < _ := by simp [eq₆, NFA.addNode]
-          . simp [Set.subset_def]
-            intro i h
-            refine .inr ⟨le_trans (NFA.le_size_of_le placeholder.property) h.left, ?_⟩
-            calc
-              i < compiled.val.nodes.size := h.right
-              _ ≤ patched.nodes.size := by simp [eq₅, eq₄]
-              _ < _ := Nat.lt_succ_self _
-        exact ⟨le_trans ih.left this, le_trans ih.right this⟩
-      | inr ge =>
-        have ge : i ≥ patched.nodes.size := by
-          simp [eq₅, eq₄]
+      have ih := ih eq₃.symm i ge size''
+      have : nfa'''[i] = nfa''.val[i] := by
+        simp [eq₅, NFA.eq_get, eq₄]
+        apply Array.get_set_ne
+        rw [eqs]
+        apply Nat.ne_of_lt
+        have : nfa.nodes.size + 1 ≤ i := by
+          simp [eq₁, NFA.addNode] at ge
           exact ge
-        have lt : i < patched.nodes.size + 1 := by
-          simp [eq, eq₆, NFA.addNode] at h₂
-          exact h₂
-        have : i = patched.nodes.size := Nat.eq_of_ge_of_lt ge lt
-        simp [eq₆, this, Node.charStep, Node.εStep]
-        simp [NFA.addNode]
-        apply Or.inr
-        apply And.intro
-        . rw [eq₂, eq₁]
-          simp [NFA.addNode]
-        . calc loopStart.val
-            _ < nodes.size := isLt'
-            _ = patched.nodes.size := by simp [eq₅, eq₄]
-            _ < _ := by simp [eq₆, NFA.addNode]
+        exact this
+      rw [this]
+      have : {start.val} ∪ NewNodesRange eq₃.symm ⊆
+        {next} ∪ {i | nfa.nodes.size ≤ i ∧ i < nfa'''.nodes.size} := by
+        apply Set.union_subset
+        . simp
+          have : start.val < nfa'''.nodes.size :=
+            calc start.val
+              _ < nfa'.val.nodes.size := start.isLt
+              _ ≤ nfa''.val.nodes.size := NFA.le_size_of_le nfa''.property
+              _ = nfa'''.nodes.size := eqsize
+          exact .inr ⟨eqs ▸ le_refl _, this⟩
+        . simp [Set.subset_def]
+          intro i h
+          exact .inr ⟨le_trans (NFA.le_size_of_le nfa'.property) h.left, eqsize ▸ h.right⟩
+      exact ⟨le_trans ih.left this, le_trans ih.right this⟩
 
 theorem compile.loop.star.lt_size (eq : compile.loop (.star r) next nfa = result) :
   nfa.nodes.size < result.val.nodes.size := by
-  apply compile.loop.star eq
-  intro placeholder loopStart compiled nodes patched final isLt isLt' property'
-    eq₁ _ eq₃ eq₄ eq₅ eq₆ eq
-
   sorry
 
-def compile.loop.star.rStart (_ : compile.loop (.star r) next nfa = result) : Nat :=
-  -- This assumes that the start node of compiled NFAs is always at the end
-  -- result.val.nodes.size - 1 is the start node of `result`, and `r` starts one node before that.
-  result.val.nodes.size - 2
+-- def compile.loop.star.rStart (_ : compile.loop (.star r) next nfa = result) : Nat :=
+--   -- This assumes that the start node of compiled NFAs is always at the end
+--   -- result.val.nodes.size - 1 is the start node of `result`, and `r` starts one node before that.
+--   result.val.nodes.size - 2
+
+-- theorem compile.loop.star.loopStartNode (eq : compile.loop (.star r) next nfa = result) :
+--   result.val[nfa.nodes.size]'(compile.loop.star.lt_size eq) = .split (compile.loop.star.rStart eq) next := by
+--   apply compile.loop.star eq
+--   intro placeholder loopStart compiled nodes patched final isLt isLt' property'
+--     eq₁ eq₂ eq₃ eq₄ eq₅ eq₆ eq'
+--   have h₁ : nfa.nodes.size < compiled.val.nodes.size :=
+--     calc nfa.nodes.size
+--       _ < placeholder.val.nodes.size := by simp [eq₁, NFA.addNode]
+--       _ ≤ _ := NFA.le_size_of_le compiled.property
+--   have h₂ : nfa.nodes.size < patched.nodes.size :=
+--     calc nfa.nodes.size
+--       _ < compiled.val.nodes.size := h₁
+--       _ = patched.nodes.size := by simp [eq₅, eq₄]
+--   have h₃ : Fin.mk loopStart isLt = ⟨nfa.nodes.size, h₁⟩ := by
+--     apply Fin.eq_of_val_eq
+--     simp [eq₂]
+--     rw [eq₁]
+--     simp [NFA.addNode]
+--   have h₄ : compiled.val.start = rStart eq := by
+--     rw [compile.loop.start eq₃.symm, rStart, eq']
+--     simp [eq₆, NFA.addNode, eq₅, eq₄]
+--   conv =>
+--     lhs
+--     simp [eq', eq₆]
+--     rw [NFA.get_lt_addNode h₂]
+--     simp [eq₅, NFA.eq_get, eq₄, h₃]
+--     rw [Array.get_set_eq]
+--     simp [h₄]
 
 theorem compile.loop.star.loopStartNode (eq : compile.loop (.star r) next nfa = result) :
-  result.val[nfa.nodes.size]'(compile.loop.star.lt_size eq) = .split (compile.loop.star.rStart eq) next := by
-  apply compile.loop.star eq
-  intro placeholder loopStart compiled nodes patched final isLt isLt' property'
-    eq₁ eq₂ eq₃ eq₄ eq₅ eq₆ eq'
-  have h₁ : nfa.nodes.size < compiled.val.nodes.size :=
-    calc nfa.nodes.size
-      _ < placeholder.val.nodes.size := by simp [eq₁, NFA.addNode]
-      _ ≤ _ := NFA.le_size_of_le compiled.property
-  have h₂ : nfa.nodes.size < patched.nodes.size :=
-    calc nfa.nodes.size
-      _ < compiled.val.nodes.size := h₁
-      _ = patched.nodes.size := by simp [eq₅, eq₄]
-  have h₃ : Fin.mk loopStart isLt = ⟨nfa.nodes.size, h₁⟩ := by
-    apply Fin.eq_of_val_eq
-    simp [eq₂]
-    rw [eq₁]
-    simp [NFA.addNode]
-  have h₄ : compiled.val.start = rStart eq := by
-    rw [compile.loop.start eq₃.symm, rStart, eq']
-    simp [eq₆, NFA.addNode, eq₅, eq₄]
-  conv =>
-    lhs
-    simp [eq', eq₆]
-    rw [NFA.get_lt_addNode h₂]
-    simp [eq₅, NFA.eq_get, eq₄, h₃]
-    rw [Array.get_set_eq]
-    simp [h₄]
+  ∃ rStart ∈ { i | nfa.nodes.size + 1 ≤ i ∧ i < result.val.nodes.size },
+  result.val[nfa.nodes.size]'(compile.loop.star.lt_size eq) = .split rStart next := sorry
+
+@[simp]
+theorem compile.loop.star.charStep_loopStartNode {c} (eq : compile.loop (.star r) next nfa = result) :
+  (result.val[nfa.nodes.size]'(compile.loop.star.lt_size eq)).charStep c = ∅ := by
+  let ⟨_, _, eq⟩ := compile.loop.star.loopStartNode eq
+  simp [eq, Node.charStep]
 
 -- TODO: prove no edge to the start
 
